src/syntax/FStarC.Syntax.Subst.fst
@@ -245,7 +245,6 @@ let subst_comp_typ' s t : ML _ =
   | [[]], NoUseRange -> t
   | _ ->
     {t with effect_name=tag_lid_with_range t.effect_name s;
-            comp_univs=List.map (subst_univ (fst s)) t.comp_univs;
             result_typ=subst' s t.result_typ;
             flags=subst_flags' s t.flags}
 
